#Example 1
Solve the equation below
$$5^{2x+7} = 125$$
Logarithms are not needed in this case.  The value on the right hand side can be expressed as a power of 5 shown below.
$$5^3 = 125$$
This allows the original equation to be manipulated into the following equivalent equation.
$$5^{2x+7} = 5^3$$
Since both sides of the equal sign share a common base, in order for equality to hold the exponents must be equal.  This translates our problem into the easier linear equation below.
$$2x+7 = 3$$
Simply solving for $x$ gives the following
$$\begin{align}
2x+7 &= 3 \\
2x &= -4 \\
x &= \frac{-4}{2} \\
x &= -2
\end{align}$$
The equation $5^{2x+1} = 125$ implies that $x=-2$.
***
#Example 2
In this example there will be more than one solution.

Solve the equation below $$3^{x^2 + 10x} = \frac{1}{9^4}$$
Logarithms are not actually needed in this case. The fraction on right side can be expressed using negative exponents.
$$3^{x^2 + 10x} = 9^{-4}$$
After manipulating the equation we see the left side of the equation has 3 as a base and the right side has 9 as a base.  Notice that $3^2=9$.  This fact will allow both sides of the equal sign to be manipulated to share a common base.
$$3^{x^2 + 10x} =\left(3^2 \right)^{-4}$$
Recall the property of exponents where $\left(a^n \right)^m = a^{n \cdot m}$.  This results in the following
$$\begin{align}
3^{x^2 + 10x} &= 3^{2 \cdot (-4)} \\
&=3^{-8}
\end{align}$$
Now our equation has a common base on both sides as shown below.
$$3^{x^2 + 10x} = 3^{-8}$$
Since both sides of the equation share a common base, the only way for equality to hold is if the exponents are equal.  This translates our equation into the problem below.
$$x^2 + 10x = -8$$
This equation is simply a quadratic that can be solved using the quadratic formula. Setting the equation in standard form gives the following
$$x^2+10x + 8 = 0$$
Using the following values
$$\begin{align}
a&=1 \\
b&= 10 \\
c&= 8
\end{align}$$
the quadratic formula gives the following solutions
$$\begin{align}
x&= \frac{-b \pm \sqrt{b^2-4ac}}{2a} \\
&=\frac{-(10) \pm\sqrt{(10)^2 - 4(1)(8)}}{2(1)} \\
&= \frac{-10 \pm\sqrt{100-32}}{2} \\
&= \frac{-10 \pm\sqrt{68}}{2} \\
&= \frac{-10 \pm 2 \sqrt{17}}{2} \\
&= -\frac{10}{2} \pm \frac{2 \sqrt{17}}{2}\\
&= -5 \pm \sqrt{17}
\end{align}$$
Now we see there are two solutions to this problem. The solutions are represented using set notation below.
$$3^{x^2 + 10x} = \frac{1}{9^4} \implies x \in \{-5+\sqrt{17} , -5-\sqrt{17}\}$$
The above expression simply states that for the equation below to be true
$$3^{x^2 + 10x} = \frac{1}{9^4}$$
it must be the case that either
$$x= -5+\sqrt{17} \;\;\;\; \text{ or } \;\;\;\; x=-5-\sqrt{17}$$
